theories/RTL/WP.v
@@ -4,11 +4,12 @@ From stdpp Require Import strings.
 From RSL Require Import Commons.Utils.
 From RSL Require Import Commons.Language.
 From RSL Require Import Commons.WP.
+From RSL Require Import Commons.NoDupDec.
+From RSL Require Import Commons.Logic.
 
 From RSL Require Import RTL.RTL.
 From RSL Require Import RTL.Notations.
 From RSL Require Import RTL.Semantics.
-From RSL Require Import RTL.Logic.
 
 Import RTLNotations.
 
@@ -171,76 +172,7 @@ Section RTLWP.
     - intros ? Hs. inv Hs. apply H with args. split.
       + eassumption.
       + apply get_regs_init_regs.
-        * apply fn_regs_no_dup.
+        * apply is_no_dup_sound. apply fn_regs_no_dup.
         * assumption.
-  Qed.
-
-  Definition NodeInv Q f pc (NI : logic) : Prop := ⊢ NI -> wp Q f pc.
-
-  Definition body : code :=
-    let x := 0 in
-    let one := 1 in
-    let ten := 2 in
-    let diff := 3 in
-    <{{
-          0: x := #0 -> 1;
-          1: one := #1 -> 2;
-          2: ten := #10 -> 3;
-          3: diff := ten - x -> 4;
-          4: if diff then goto 6 else goto 5;
-          5: x := x + one -> 3;
-          6: ret x;
-      }}>.
-
-  Definition test : function :=
-    {|
-      fn_name := "test"%string;
-      fn_regs := [];
-      fn_entrypoint := 0;
-      fn_code := body;
-      fn_regs_no_dup := NoDup_nil_2;
-    |}.
-
-  Ltac step lemma :=
-    match goal with
-    | |- wp _ ?f ?pc _ _ ?n =>
-        let H := fresh "Hpc" in
-        eassert (H: f@pc is _) by reflexivity;
-        eapply lemma;
-        [now apply H|];
-        clear H; repeat split; simpl_reg; unfold_Prop; simpl;
-        try (destruct n as [|n]; [easy|])
-    | |- match ?n with
-         | O => True
-         | S n' => wp _ _ _ _ _ n'
-         end => destruct n as [|n]; [easy|step lemma]
-    end.
-
-  Lemma test_inv :
-    NodeInv (fun v m => v = 10%Z) test 3
-      ⟨1 ↦ᵣ 1%Z ∧ 2 ↦ᵣ 10%Z ∧ ∃ v, 0 ↦ᵣ v ∧ ⌜(v <= 10)%Z⌝⟩.
-  Proof.
-    apply löb.
-    intros ρ m n IH (Hone & Hten & v & Hres & Hv).
-    step wp_op.
-    step wp_cond.
-    destruct (10 - v =? 0)%Z eqn:He.
-    - step wp_ret. repeat split. simpl_reg.
-    - step wp_op. eapply safe_mono; [|apply IH].
-      + lia.
-      + simpl_reg. eexists. repeat split.
-        lia.
-  Qed.
-
-  Lemma test_correct :
-    hoare (fun args m => True) test (fun v m => v = 10%Z).
-  Proof.
-    apply hoare_from_wp.
-    intros args ρ m n _.
-    step wp_op.
-    step wp_op.
-    step wp_op.
-    apply test_inv. repeat (simpl_reg; unfold_Prop).
-    eexists. repeat split. lia.
   Qed.
 End RTLWP.
