theories/Commons/Definitions.v
@@ -1,0 +1,53 @@
+From stdpp Require Import prelude.
+From stdpp Require Import strings.
+From stdpp Require Import gmap.
+
+Definition ident : Type := string.
+Definition val : Type := Z.
+
+Definition node := nat.
+Definition loc := positive.
+Definition reg := nat.
+
+(* [regmap] is a mapping from registers to a value *)
+Definition regmap : Type := gmap reg val.
+
+(* [memory] is a mapping from location to a value *)
+Definition memory : Type := gmap loc val.
+
+Definition loc_to_val (l: loc) : val := Zpos l.
+
+Definition val_to_loc (v: val) : option loc :=
+  if (v >=? 1)%Z
+  then Some (Z.to_pos v)
+  else None.
+
+Definition get_reg (r: reg) (ρ: regmap) : val :=
+  match ρ !! r with
+  | Some v => v
+  | None => 0%Z (* Dummy val *)
+  end.
+
+Definition get_regs (l: list reg) (ρ: regmap) : list val :=
+  map (fun r => get_reg r ρ) l.
+
+Definition set_reg (r: reg) (v: val) (ρ: regmap) : regmap := <[r := v]>ρ.
+
+Definition get_at (addr: val) (m: memory) : option val :=
+  match val_to_loc addr with
+  | Some loc => m !! loc
+  | None => None
+  end.
+
+Definition update_at (addr: val) (f: val -> val) (m: memory) : option memory
+  := match val_to_loc addr with
+     | Some loc =>
+         match m !! loc with
+         | Some old => Some (<[loc := f old]>m)
+         | None => None
+         end
+     | None => None
+     end.
+
+Definition set_at (addr: val) (v: val) (m: memory) : option memory :=
+  update_at addr (fun _ => v) m.
