theories/Commons/NoDupDec.v
@@ -1,0 +1,47 @@
+From stdpp Require Import prelude.
+
+Section no_dup.
+  Context `{dec : EqDecision A}.
+
+  Global Instance list_elem_of_dec : RelDecision (∈@{list A}).
+  Proof using Type*.
+   refine (
+    fix go x l :=
+    match l return Decision (x ∈ l) with
+    | [] => right _
+    | y :: l => cast_if_or (decide (x = y)) (go x l)
+    end); clear go dec; subst; try (by constructor); abstract by inv 1.
+  Defined.
+
+  Fixpoint is_no_dup (l: list A) : bool :=
+    match l with
+    | [] => true
+    | hd :: tl =>
+        if decide_rel (∈) hd tl
+        then false
+        else is_no_dup tl
+    end.
+
+  Lemma is_no_dup_sound:
+    ∀ l, is_no_dup l = true <-> NoDup l.
+  Proof.
+    intros l. induction l as [ | hd tl IH ].
+    - split; constructor.
+    - simpl; destruct (decide_rel elem_of hd tl) as [He | Hne].
+      + split; intro H.
+        * discriminate H.
+        * exfalso. inv H as [ | ? ? Hne ]. now apply Hne.
+      + split; intro H.
+        * constructor; auto. now apply IH.
+        * apply IH. now inv H.
+  Qed.
+
+  Lemma no_dup_dec : ∀ l : list A, Decision (NoDup l).
+  Proof.
+    intros l. destruct (is_no_dup l) eqn:H.
+    - left. now apply is_no_dup_sound.
+    - right. intro HD.
+      apply is_no_dup_sound in HD.
+      congruence.
+  Qed.
+End no_dup.
