theories/RTL/Playground.v
@@ -1,0 +1,88 @@
+From stdpp Require Import prelude.
+From stdpp Require Import strings.
+
+From RSL Require Import Commons.Utils.
+From RSL Require Import Commons.Language.
+From RSL Require Import Commons.WP.
+From RSL Require Import Commons.NoDupDec.
+From RSL Require Import Commons.Logic.
+
+From RSL Require Import RTL.RTL.
+From RSL Require Import RTL.Semantics.
+From RSL Require Import RTL.Notations.
+From RSL Require Import RTL.WP.
+
+Import RTLNotations.
+
+Section Play.
+  Let Λ : lang := rtl_lang.
+  Context (P: prog Λ).
+
+  Let x : reg := 0.
+  Let one : reg := 1.
+  Let ten : reg := 2.
+  Let diff : reg := 3.
+
+  Definition NodeInv Q f pc (NI : logic) : Prop := ⊢ NI -> wp P Q f pc.
+
+  Definition test : function :=
+    {|
+      fn_name := "test"%string;
+      fn_regs := [];
+      fn_entrypoint := 0;
+      fn_code := <{{
+            0: x := #0 -> 1;
+            1: one := #1 -> 2;
+            2: ten := #10 -> 3;
+            3: diff := ten - x -> 4;
+            4: if diff then goto 6 else goto 5;
+            5: x := x + one -> 3;
+            6: ret x;
+        }}>;
+      fn_regs_no_dup := eq_refl;
+    |}.
+
+  Ltac step lemma :=
+    match goal with
+    | |- wp _ _ ?f ?pc _ _ ?n =>
+        let H := fresh "Hpc" in
+        eassert (H: f@pc is _) by reflexivity;
+        eapply lemma;
+        [now apply H|];
+        clear H; repeat split; simpl_reg; unfold_Prop; simpl;
+        try (destruct n as [|n]; [easy|])
+    | |- match ?n with
+         | O => True
+         | S n' => wp _ _ _ _ _ _ n'
+         end => destruct n as [|n]; [easy|step lemma]
+    end.
+
+  Lemma test_inv :
+    NodeInv (fun v m => v = 10%Z) test 3
+      ⟨one ↦ᵣ 1%Z ∧ ten ↦ᵣ 10%Z ∧ ∃ v, x ↦ᵣ v ∧ ⌜(v <= 10)%Z⌝⟩.
+  Proof.
+    apply löb.
+    intros ρ m n IH (Hone & Hten & v & Hres & Hv).
+    step wp_op.
+    step wp_cond.
+    destruct (10 - v =? 0)%Z eqn:He.
+    - step wp_ret. repeat split. simpl_reg.
+    - step wp_op. eapply safe_mono; [|apply IH].
+      + lia.
+      + simpl_reg. eexists. repeat split.
+        lia.
+  Qed.
+
+  Lemma test_correct :
+    hoare P (fun args m => True) test (fun v m => v = 10%Z).
+  Proof.
+    apply hoare_from_wp.
+    intros args ρ m n _.
+    step wp_op.
+    step wp_op.
+    step wp_op.
+    apply test_inv. repeat (simpl_reg; unfold_Prop).
+    eexists. repeat split. lia.
+  Qed.
+
+End Play.
