theories/Toy/Compile.v
@@ -1,0 +1,100 @@
+From stdpp Require Import prelude.
+
+From RSL Require Import RTL.RTL.
+From RSL Require Import Toy.Toy.
+
+Definition Build (T: Type) : Type :=
+  node -> option (node * T * code).
+
+Instance build_bind : MBind Build :=
+  fun _ _ f m pc =>
+    '(pc, x, c1) ← m pc;
+    '(pc, y, c2) ← f x pc;
+    mret (pc, y, c1 ∪ c2).
+
+Instance build_ret : MRet Build :=
+  fun _ x pc => Some (pc, x, ∅).
+
+Instance build_fail : MFail Build :=
+  fun _ _ _ => None.
+
+Definition add (i: instr) : Build node :=
+  fun pc =>
+    let next_pc := 1 + pc in
+    Some (1 + pc, pc, {[ pc := i ]}).
+
+Definition add_next (npc: option node) (i: node -> instr) : Build node :=
+  match npc with
+  | Some npc => add $ i npc
+  | None => mfail
+  end.
+
+Definition reserve : Build (node * (instr -> Build unit)) :=
+  fun reserved_pc =>
+    let fill (i: instr) : Build unit :=
+      fun current_pc => Some (current_pc, (), {[ reserved_pc := i ]})
+    in
+    Some (1 + reserved_pc, (reserved_pc, fill), ∅).
+
+Definition texpr_rtl (dst: reg) (e: texpr) (npc: node) : instr :=
+  match e with
+  | EReg r => Iop Move [r] dst npc
+  | EImm v => Iop (LoadI v) [] dst npc
+  | ELoad addr => Iload addr dst npc
+  | EAdd lhs rhs => Iop Add [lhs; rhs] dst npc
+  | ESub lhs rhs => Iop Sub [lhs; rhs] dst npc
+  | EMul lhs rhs => Iop Mul [lhs; rhs] dst npc
+  end.
+
+Fixpoint tinstr_rtl (i: tinstr) (npc: option node) (bpc: list node) : Build node :=
+  match i with
+  | ISkip =>
+      add_next npc $ Inop
+
+  | IBreak level =>
+      add_next (bpc !! level) $ Inop
+
+  | IRet v =>
+      add $ Ireturn v
+
+  | ICall dst name args =>
+      add_next npc $ Icall name args dst
+
+  | IAssign dst e =>
+      add_next npc $ texpr_rtl dst e
+
+  | IStore addr e =>
+      add_next npc $ Istore addr e
+
+  | ISeq fst snd =>
+      npc_snd ← tinstr_rtl snd npc bpc;
+      tinstr_rtl fst (Some npc_snd) bpc
+
+  | IIf cond trueB falseB =>
+      npc_true ← tinstr_rtl trueB npc bpc;
+      npc_false ← tinstr_rtl falseB npc bpc;
+      add $ Icond cond npc_true npc_false
+
+  | ILoop body rest =>
+      npc_rest ← tinstr_rtl rest npc bpc;
+      '(loop_init, cb) ← reserve;
+      loop_fst ← tinstr_rtl body (Some loop_init) (npc_rest :: bpc);
+      '() ← cb (Inop loop_fst);
+      mret loop_fst
+  end.
+
+Definition compile (f: tfunction) : option function :=
+  let c := tfn_code f in
+  match tinstr_rtl c None [] 0 with
+  | None =>
+      None
+  | Some (_, entry, c) =>
+      Some
+        {|
+          fn_name := tfn_name f;
+          fn_regs := tfn_regs f;
+          fn_entrypoint := entry;
+          fn_code := c;
+          fn_regs_no_dup := tfn_regs_no_dup f;
+        |}
+  end.
