theories/Toy/Notations.v
@@ -1,0 +1,112 @@
+From stdpp Require Import prelude.
+
+From RSL Require Import Toy.Toy.
+
+Module ToyNotations.
+  Declare Custom Entry toy_instr.
+  Declare Custom Entry toy_expr.
+  Declare Custom Entry toy_reg.
+
+  Notation "<{| e |}>" := e (e custom toy_instr at level 99).
+
+  Notation "r" :=
+    (EReg r)
+      (in custom toy_expr at level 0,
+          r ident).
+
+  Notation "# v" :=
+    (EImm v%Z)
+      (in custom toy_expr at level 0,
+          v constr).
+
+  Notation "'!' addr" :=
+    (ELoad addr)
+      (in custom toy_expr at level 0,
+          addr ident).
+
+  Notation "x '*' y" :=
+    (EMul x y)
+      (in custom toy_expr at level 0,
+          x ident,
+          y ident,
+          left associativity).
+
+  Notation "x '+' y" :=
+    (EAdd x y)
+      (in custom toy_expr at level 0,
+          x ident,
+          y ident,
+          left associativity).
+
+  Notation "x '-' y" :=
+    (ESub x y)
+      (in custom toy_expr at level 0,
+          x ident,
+          y ident,
+          left associativity).
+
+  Notation "'skip'" :=
+    ISkip
+      (in custom toy_instr).
+
+  Notation "'break' n" :=
+    (IBreak n)
+      (in custom toy_instr at level 10,
+          n constr).
+
+  Notation "'return' v" :=
+    (IRet v)
+      (in custom toy_instr at level 10,
+          v ident).
+
+  Notation "dst ':=' '@' f '(' args ')'" :=
+    (ICall dst f args)
+      (in custom toy_instr at level 0,
+          dst ident,
+          f ident,
+          args constr).
+
+  Notation "dst ':=' e" :=
+    (IAssign dst e)
+      (in custom toy_instr at level 0,
+          dst ident,
+          e custom toy_expr).
+
+  Notation "'*' addr ':=' r" :=
+    (IStore addr r)
+      (in custom toy_instr at level 70,
+          addr ident,
+          r ident).
+
+  Notation "'if' cond '{' b1 '}' 'else' '{' b2 '}'" :=
+    (IIf cond b1 b2)
+      (in custom toy_instr at level 80,
+          cond ident,
+          b1 custom toy_instr,
+          b2 custom toy_instr).
+
+  Notation "'loop' '{' b '}'" :=
+    (ILoop b ISkip)
+      (in custom toy_instr at level 80,
+          b custom toy_instr).
+
+  Notation "'while' cond '{' b '}'" :=
+    (IWhile cond b)
+      (in custom toy_instr at level 80,
+          cond ident,
+          b custom toy_instr).
+
+  Notation "'do' '{' b '}' 'while' cond" :=
+    (IDoWhile b cond)
+      (in custom toy_instr at level 80,
+          b ident,
+          cond custom toy_reg).
+
+  Notation "s1 ; s2" :=
+    (ISeq s1 s2)
+      (in custom toy_instr at level 90,
+          s1 custom toy_instr,
+          s2 custom toy_instr,
+          right associativity).
+
+End ToyNotations.
