theories/Toy/Toy.v
@@ -1,0 +1,36 @@
+From stdpp Require Import prelude.
+
+From RSL Require Export Commons.Definitions.
+From RSL Require Import Commons.NoDupDec.
+
+Variant texpr : Type :=
+| EReg (r: reg)
+| EImm (v: val)
+| ELoad (addr: reg)
+| EAdd (lhs rhs: reg)
+| ESub (lhs rhs: reg)
+| EMul (lhs rhs: reg).
+
+Inductive tinstr : Type :=
+| ISkip
+| IBreak (level: nat)
+| IRet (v: reg)
+| ICall (dst: reg) (name: ident) (args: list reg)
+| ISeq (fst snd: tinstr)
+| IAssign (dst: reg) (e: texpr)
+| IStore  (addr: reg) (e: reg)
+| IIf (cond: reg) (trueB falseB: tinstr)
+| ILoop (body: tinstr) (rest: tinstr).
+
+Definition IWhile (cond: reg) (body: tinstr) : tinstr :=
+  ILoop (ISeq (IIf cond ISkip (IBreak 0)) body) ISkip.
+
+Definition IDoWhile (body: tinstr) (cond: reg) : tinstr :=
+  ILoop (ISeq body (IIf cond ISkip (IBreak 0))) ISkip.
+
+Record tfunction := {
+    tfn_name: ident;
+    tfn_regs: list reg;
+    tfn_code : tinstr;
+    tfn_regs_no_dup : is_no_dup tfn_regs = true;
+  }.
